Rename Debug options to Flag options
h/t Andres

This will let us reuse them for rewrite passes without me feeling silly about naming.

src/Util/Strings/ParseFlagOptions.v
@@ -13,33 +13,33 @@ Local Open Scope string_scope.
 Local Set Boolean Equality Schemes.
 Local Set Decidable Equality Schemes.
 
-Variant debug_status := enabled | disabled.
-Variant full_debug_status := explicit (_ : debug_status) | elided.
-Global Coercion explicit : debug_status >-> full_debug_status.
-Coercion bool_of_debug_status (d : debug_status) : bool
+Variant flag_status := enabled | disabled.
+Variant full_flag_status := explicit (_ : flag_status) | elided.
+Global Coercion explicit : flag_status >-> full_flag_status.
+Coercion bool_of_flag_status (d : flag_status) : bool
   := match d with
      | enabled => true
      | disabled => false
      end.
-Definition bool_of_full_debug_status (d : full_debug_status) (default : bool) : bool
+Definition bool_of_full_flag_status (d : full_flag_status) (default : bool) : bool
   := match d with
      | elided => default
-     | explicit d => bool_of_debug_status d
+     | explicit d => bool_of_flag_status d
      end.
-Global Instance show_debug_status : Show debug_status
+Global Instance show_flag_status : Show flag_status
   := fun s => match s with
               | enabled => "enabled"
               | disabled => "disabled"
               end.
-Global Instance show_full_debug_status : Show full_debug_status
+Global Instance show_full_flag_status : Show full_flag_status
   := fun s => match s with
               | explicit s => show s
               | elided => "elided"
               end.
-Variant debug_option_kind := all | alias (_ : list string).
-Coercion simple (s : string) : debug_option_kind := alias [s].
+Variant flag_option_kind := all | alias (_ : list string).
+Coercion simple (s : string) : flag_option_kind := alias [s].
 
-Definition preparse_debug_opts (spec : list (string * debug_option_kind)) (args : list string) : list (debug_option_kind * debug_status)
+Definition preparse_flag_opts (spec : list (string * flag_option_kind)) (args : list string) : list (flag_option_kind * flag_status)
   := let spec := List.fold_left (fun acc '(s, k) => StringMap.add s k acc) spec (@StringMap.empty _) in
      let args := List.filter (fun s => negb (s =? "")) (List.map String.trim (List.flat_map (String.split ",") args)) in
      List.map
@@ -53,7 +53,7 @@ Definition preparse_debug_opts (spec : list (string * debug_option_kind)) (args 
            (Option.value (StringMap.find arg spec) (simple arg), status))
        args.
 
-Definition aggregate_debug_opts (args : list (debug_option_kind * debug_status)) : full_debug_status (* all status *) * StringMap.t debug_status
+Definition aggregate_flag_opts (args : list (flag_option_kind * flag_status)) : full_flag_status (* all status *) * StringMap.t flag_status
   := List.fold_left
        (fun '(all_status, acc) '(k, s)
         => match k with
@@ -68,8 +68,8 @@ Definition aggregate_debug_opts (args : list (debug_option_kind * debug_status))
        args
        (elided, @StringMap.empty _).
 
-Fixpoint format_debug_opts (known_options : list string) (status : StringMap.t debug_status) : Tuple.tuple full_debug_status (List.length known_options)
-  := match known_options return Tuple.tuple full_debug_status (List.length known_options) with
+Fixpoint format_flag_opts (known_options : list string) (status : StringMap.t flag_status) : Tuple.tuple full_flag_status (List.length known_options)
+  := match known_options return Tuple.tuple full_flag_status (List.length known_options) with
      | [] => tt
      | opt :: opts
        => Tuple.cons
@@ -77,19 +77,19 @@ Fixpoint format_debug_opts (known_options : list string) (status : StringMap.t d
             | Some s => explicit s
             | None => elided
             end
-            (format_debug_opts opts status)
+            (format_flag_opts opts status)
      end.
 
-Definition post_parse_debug_opts (known_options : list string) (status : full_debug_status (* all status *) * StringMap.t debug_status)
-  : full_debug_status (* all status *) * list (string * debug_status) (* unknown options *) * Tuple.tuple full_debug_status (List.length known_options)
+Definition post_parse_flag_opts (known_options : list string) (status : full_flag_status (* all status *) * StringMap.t flag_status)
+  : full_flag_status (* all status *) * list (string * flag_status) (* unknown options *) * Tuple.tuple full_flag_status (List.length known_options)
   := let '(all_status, status) := status in
      let known_options_set := List.fold_right StringSet.add StringSet.empty known_options in
      let unknown_options := List.filter (fun '(opt, _) => negb (StringSet.mem opt known_options_set)) (StringMap.elements status) in
-     (all_status, unknown_options, format_debug_opts known_options status).
+     (all_status, unknown_options, format_flag_opts known_options status).
 
-Definition parse_debug_opts (spec : list (string * debug_option_kind)) (known_options : list string) (args : list string)
-  : full_debug_status (* all status *) * list (string * debug_status) (* unknown options *) * Tuple.tuple full_debug_status (List.length known_options)
-  := let res := preparse_debug_opts spec args in
-     let res := aggregate_debug_opts res in
-     let res := post_parse_debug_opts known_options res in
+Definition parse_flag_opts (spec : list (string * flag_option_kind)) (known_options : list string) (args : list string)
+  : full_flag_status (* all status *) * list (string * flag_status) (* unknown options *) * Tuple.tuple full_flag_status (List.length known_options)
+  := let res := preparse_flag_opts spec args in
+     let res := aggregate_flag_opts res in
+     let res := post_parse_flag_opts known_options res in
      res.
