src/StandaloneDebuggingExamples.v
@@ -25,7 +25,7 @@ Module debugging_no_asm.
     cbv [ForExtraction.parse_common_optional_options] in v.
     cbv [ForExtraction.hint_file_names] in v.
     cbn [map fst snd] in v.
-    vm_compute ParseDebugOptions.parse_debug_opts in v.
+    vm_compute ParseFlagOptions.parse_flag_opts in v.
     cbv beta iota in v.
     cbn [ForExtraction.with_read_concat_asm_files_cps] in v.
     set (k := ForExtraction.with_read_file "t.asm") in (value of v).
@@ -124,7 +124,7 @@ Module debugging_typedef_bounds.
     cbv [ForExtraction.parse_common_optional_options] in v.
     cbv [ForExtraction.hint_file_names] in v.
     cbn [map] in v.
-    vm_compute ParseDebugOptions.parse_debug_opts in v.
+    vm_compute ParseFlagOptions.parse_flag_opts in v.
     cbv beta iota in v.
     cbn [ForExtraction.with_read_concat_asm_files_cps] in v.
     vm_compute ForExtraction.parse_args in v.
